some cleanup + make Inode.v use RecArray.v

src/Inode.v
@@ -27,7 +27,7 @@ Set Implicit Arguments.
 
 Record xparams := {
   IXStart : addr;
-    IXLen : addr
+  IXLen : addr
 }.
 
 Module INODE.
@@ -41,7 +41,7 @@ Module INODE.
 
   Definition itemsz := Rec.len inodetype.
   Definition items_per_valu : addr := $16.
-  Theorem itemsz_ok : wordToNat items_per_valu * itemsz = valulen.
+  Theorem itemsz_ok : valulen = wordToNat items_per_valu * itemsz.
   Proof.
     rewrite valulen_is; auto.
   Qed.
@@ -54,258 +54,19 @@ Module INODE.
     rewrite valulen_is; auto.
   Qed.
 
+  Definition xp_to_raxp xp :=
+    RecArray.Build_xparams (IXStart xp) (IXLen xp).
 
-  Definition rep_block (b : block) : valu.
-    rewrite <- blocksz. apply (Rec.to_word b).
-  Defined.
-
-  Definition valu_to_block (v : valu) : block.
-    rewrite <- blocksz in v. apply (Rec.of_word v).
-  Defined.
-
-  Lemma rep_valu_id : forall b, Rec.well_formed b -> valu_to_block (rep_block b) = b.
-    unfold valu_to_block, rep_block.
-    unfold eq_rec_r, eq_rec.
-    intros.
-    rewrite Pack.eq_rect_nat_double.
-    rewrite <- eq_rect_eq_dec; [| apply eq_nat_dec ].
-    apply Rec.of_to_id; assumption.
-  Qed.
-
-  (** The representation invariant for the first layer, which uses two indices *)
-  Definition rep_pair xp (ilistlist : list block) :=
-    ([[ length ilistlist = wordToNat (IXLen xp) ]] *
-     [[ Forall Rec.well_formed ilistlist ]] *
-     array (IXStart xp)
-          (map (fun i => rep_block (selN ilistlist i nil))
-          (seq 0 (wordToNat (IXLen xp)))) $1)%pred.
-
-  (** Get the [ipos]'th inode in the [iblock]'th block *)
-  Definition iget_pair T lxp xp iblock ipos rx : prog T :=
-    v <- LOG.read_array lxp (IXStart xp) iblock $1 ;
-    let ib := valu_to_block v in
-    let i := sel ib ipos inode_zero in
-    rx i.
-
-  (** Update the [ipos]'th inode in the [iblock]'th block to [i] *)
-  Definition iput_pair T lxp xp iblock ipos i rx : prog T :=
-    v <- LOG.read_array lxp (IXStart xp) iblock $1 ;
-    let ib' := upd (valu_to_block v) ipos i in
-    let v' := rep_block ib' in
-    ok <- LOG.write_array lxp (IXStart xp) iblock $1 v' ;
-    rx ok.
-
-  Hint Rewrite map_length.
-  Hint Rewrite seq_length.
-  Hint Resolve wlt_lt.
-  Hint Rewrite sel_map_seq using auto.
-  Hint Rewrite rep_valu_id.
-
-  (** Not sure why we didn't just use [nth] *)
-  Lemma nth_selN_eq : forall t n l (z:t), selN l n z = nth n l z.
-  Proof.
-    induction n; intros; destruct l; simpl; auto.
-  Qed.
-
-  Ltac nth_selN H := intros; repeat rewrite nth_selN_eq; apply H; assumption.
-
-  Lemma in_selN : forall t n l (z:t), n < length l -> In (selN l n z) l.
-  Proof.
-    nth_selN nth_In.
-  Qed.
-
-  Lemma in_sel : forall t n l (z:t), wordToNat n < length l -> In (sel l n z) l.
-  Proof.
-    intros. apply in_selN; assumption.
-  Qed.
-
-  Theorem iget_pair_ok : forall lxp xp iblock ipos,
-    {< F mbase m ilistlist,
-    PRE    LOG.rep lxp (ActiveTxn mbase m) *
-           [[ (F * rep_pair xp ilistlist)%pred m ]] *
-           [[ (iblock < IXLen xp)%word ]] *
-           [[ (ipos < items_per_valu)%word ]]
-    POST:r LOG.rep lxp (ActiveTxn mbase m) *
-           [[ r = sel (sel ilistlist iblock nil) ipos inode_zero ]]
-    CRASH  LOG.log_intact lxp mbase
-    >} iget_pair lxp xp iblock ipos.
-  Proof.
-    unfold iget_pair.
-    hoare.
-    unfold rep_pair in *. cancel.
-    autorewrite with core. auto.
-
-    subst. autorewrite with core. auto.
-    unfold rep_pair in H3.
-    destruct_lift H3. rewrite Forall_forall in H9. apply H9.
-    apply in_selN. rewrite H7. auto.
-    unfold LOG.log_intact. cancel.
-  Qed.
-
-  Lemma selS : forall t (z : t) h l i,
-    selN l i z = selN (h :: l) (S i) z.
-  Proof.
-    auto.
-  Qed.
-
-  Lemma sel_lists_eq : forall t (z : t) n l1 l2, n = length l1 -> n = length l2 ->
-    (forall i, i < n -> selN l1 i z = selN l2 i z) -> l1 = l2.
-  Proof.
-    induction n; destruct l1; try discriminate; destruct l2; try discriminate.
-    trivial.
-    intros.
-    replace t1 with t0 by (apply (H1 0); omega).
-    replace l2 with l1. trivial. apply IHn; auto.
-    intros i Hl. erewrite selS.
-    replace (selN l2 i z) with (selN (t1 :: l2) (S i) z). apply H1. omega.
-    erewrite <- selS. trivial.
-  Qed.
-
-  (** Mapping indexing into l over the list of indices in l gives you l *)
-  Lemma map_sel_seq : forall t (z : t) (l : list t) n,
-    n = length l -> map (fun i => selN l i z) (seq 0 n) = l.
-  Proof.
-    intros. apply sel_lists_eq with (z := z) (n := n); auto.
-    rewrite map_length. rewrite seq_length. trivial.
-    intros i Hl. apply selN_map_seq; assumption.
-  Qed.
-
-  Theorem iput_update : forall xlen inode l iblock ipos,
-    (ipos < items_per_valu)%word ->
-    xlen = length l ->
-    (upd (map (fun i => rep_block (selN l i nil)) (seq 0 xlen)) iblock
-       (rep_block (upd (selN l (wordToNat iblock) nil) ipos inode))) =
-    (map (fun i => rep_block (selN (upd l iblock (upd (sel l iblock nil) ipos inode)) i nil))
-       (seq 0 xlen)).
-  Proof.
-    unfold upd, sel; intros. remember (updN (selN l (wordToNat iblock) nil) (wordToNat ipos) inode0) as ud.
-    rewrite <- map_map. rewrite map_sel_seq by assumption. rewrite <- map_updN.
-    replace (map (fun i : nat => rep_block (selN (updN l (wordToNat iblock) ud) i nil)) (seq 0 xlen))
-      with (map rep_block (map (fun i : nat => (selN (updN l (wordToNat iblock) ud) i nil)) (seq 0 xlen)))
-      by (apply map_map). (* XXX how can I specify the rewrite location here?? *)
-    rewrite map_sel_seq. trivial. autorewrite with core. assumption.
-  Qed.
-
-  Lemma in_updN : forall t n l x (xn:t), In x (updN l n xn) ->
-    In x l \/ x = xn.
-  Proof.
-    induction n; intros; destruct l; intuition; simpl in *; destruct H; auto.
-    destruct (IHn l x xn H); auto.
-  Qed.
-
-  Lemma in_upd : forall t n l x (xn:t), In x (upd l n xn) ->
-    In x l \/ x = xn.
-  Proof.
-    intros. apply in_updN with (n:=wordToNat n); auto.
-  Qed.
-
-  Lemma Forall_upd : forall t P l n (v:t), Forall P l -> P v -> Forall P (upd l n v).
-  Proof.
-    intros. apply Forall_forall. intros v0 Hi. apply in_upd in Hi. destruct Hi.
-    rewrite Forall_forall in H. apply H; assumption.
-    subst. assumption.
-  Qed.
-
-  Theorem iput_pair_ok : forall lxp xp iblock ipos i,
-    {< F mbase m ilistlist,
-    PRE    LOG.rep lxp (ActiveTxn mbase m) *
-           [[ (F * rep_pair xp ilistlist)%pred m ]] *
-           [[ (iblock < IXLen xp)%word ]] *
-           [[ (ipos < items_per_valu)%word ]] *
-           [[ Rec.well_formed i ]]
-    POST:r ([[ r = false ]] * LOG.rep lxp (ActiveTxn mbase m)) \/
-           ([[ r = true ]] * exists m', LOG.rep lxp (ActiveTxn mbase m') *
-            [[ (F * rep_pair xp (upd ilistlist iblock (upd (sel ilistlist iblock nil) ipos i)))%pred m' ]])
-    CRASH  LOG.log_intact lxp mbase
-    >} iput_pair lxp xp iblock ipos i.
-  Proof.
-    unfold iput_pair.
-    hoare_unfold LOG.unfold_intact.
-    unfold rep_pair. cancel.
-    autorewrite with core. auto.
-    unfold rep_pair. cancel.
-
-    (* Coq bug 3815 or 3816? *)
-    autorewrite with core. auto.
-
-    apply pimpl_or_r. right. unfold rep_pair in *.
-    destruct_lift H. cancel.
-    rewrite sel_map_seq by auto. autorewrite with core.
-    rewrite iput_update; auto.
-    rewrite Forall_forall in H9. apply H9.
-    apply in_selN. rewrite H7. auto.
-    autorewrite with core. auto.
-    apply Forall_upd. assumption.
-    split. autorewrite with core. rewrite Forall_forall in H9. apply H9.
-    apply in_sel. rewrite H7. auto.
-    apply Forall_upd. rewrite Forall_forall in H9. apply H9. apply in_sel. rewrite H7. auto.
-    rewrite Forall_forall in H9.
-    auto.
-  Qed.
-
-
-  Hint Extern 1 ({{_}} progseq (iget_pair _ _ _ _) _) => apply iget_pair_ok : prog.
-  Hint Extern 1 ({{_}} progseq (iput_pair _ _ _ _ _) _) => apply iput_pair_ok : prog.
-
-  (** The representation invariant for the second layer, which uses one index *)
   Definition rep xp (ilist : list inode) :=
-    (exists ilistlist, rep_pair xp ilistlist *
-     [[ ilist = fold_right (@app _) nil ilistlist ]])%pred.
+    RecArray.array_item inodetype items_per_valu itemsz_ok (xp_to_raxp xp) ilist.
 
   Definition iget T lxp xp inum rx : prog T :=
-    i <- iget_pair lxp xp (inum ^/ items_per_valu) (inum ^% items_per_valu);
-    rx i.
+    RecArray.get inodetype items_per_valu itemsz_ok
+      lxp (xp_to_raxp xp) inum rx.
 
   Definition iput T lxp xp inum i rx : prog T :=
-    ok <- iput_pair lxp xp (inum ^/ items_per_valu) (inum ^% items_per_valu) i;
-    rx ok.
-
-  Lemma selN_app1 : forall t l l' (d:t) n,
-    n < length l -> selN (l ++ l') n d = selN l n d.
-  Proof.
-    nth_selN app_nth1.
-  Qed.
-
-  Lemma selN_app2 : forall t l l' (d:t) n,
-    n >= length l -> selN (l ++ l') n d = selN l' (n - length l) d.
-  Proof.
-    nth_selN app_nth2.
-  Qed.
-
-  Lemma nested_selN_concat : forall t a b m l (z:t), b < m ->
-    Forall (fun sl => length sl = m) l ->
-    selN (selN l a nil) b z = selN (fold_right (app (A:=t)) nil l) (b + a * m) z.
-  Proof.
-    induction a; intros; destruct l; simpl; inversion H0.
-    trivial.
-    replace (b + 0) with b by omega. subst.
-    rewrite selN_app1; auto.
-    trivial.
-    subst. remember (a * length l) as al. rewrite selN_app2 by omega.
-    replace (b + (length l + al) - length l) with (b + al) by omega. subst.
-    apply IHa; assumption.
-  Qed.
-
-  (** If we index into the concatenation of a list of length-[m] lists, it's
-      the same as indexing into the [n % m]'th element of the [n / m]'th list *)
-  Lemma nested_sel_divmod_concat : forall t l n m (z:t), m <> $0 ->
-    Forall (fun sl => length sl = wordToNat m) l ->
-    sel (sel l (n ^/ m) nil) (n ^% m) z = sel (fold_right (app (A:=t)) nil l) n z.
-  Proof.
-    intros. unfold sel. rewrite nested_selN_concat with (m:=wordToNat m).
-    word2nat'. rewrite Nat.mul_comm. rewrite Nat.add_comm. rewrite <- Nat.div_mod.
-    trivial. assumption. apply le_lt_trans with (m := wordToNat n). apply div_le; assumption.
-    apply wordToNat_bound.
-    apply lt_le_trans with (m := wordToNat m).
-    apply Nat.mod_upper_bound; assumption.
-    apply Nat.lt_le_incl; apply wordToNat_bound.
-    word2nat'.
-    apply Nat.mod_upper_bound; assumption.
-    apply lt_le_trans with (m := wordToNat m).
-    apply Nat.mod_upper_bound; assumption.
-    apply Nat.lt_le_incl; apply wordToNat_bound.
-    assumption.
-  Qed.
+    RecArray.put inodetype items_per_valu itemsz_ok
+      lxp (xp_to_raxp xp) inum i rx.
 
   Theorem iget_ok : forall lxp xp inum,
     {< F mbase m ilist,
@@ -318,28 +79,7 @@ Module INODE.
     >} iget lxp xp inum.
   Proof.
     unfold iget, rep.
-
-    intros.
-    eapply pimpl_ok2. eauto with prog.
-
-    intros.
-    norm.
-    cancel.
-    (* Something about type coersions is making [assumption] take forever.. *)
-    split; [constructor |].
-    split; [constructor |].
-    split; [constructor |].
-    split; [constructor |].
-    pred_apply; instantiate (a2:=l); cancel.
-    apply wdiv_lt_upper_bound; [word_neq | rewrite wmult_comm; assumption].
-    apply wmod_upper_bound; word_neq.
-    step.
-    subst.
-    unfold rep_pair in H. unfold rep_block in H.
-    rewrite H9. destruct_lift H.
-    apply nested_sel_divmod_concat; auto. word_neq.
-    eapply Forall_impl; [| apply H8].
-    intro a. simpl. tauto.
+    intros. eapply pimpl_ok2. eapply RecArray.get_ok; word_neq.
     step.
   Qed.
 
@@ -356,38 +96,8 @@ Module INODE.
     >} iput lxp xp inum i.
   Proof.
     unfold iput, rep.
-    intros. eapply pimpl_ok2. eauto with prog.
-    intros.
-    norm.
-    cancel.
-    split; [constructor |].
-    split; [constructor |].
-    split; [constructor |].
-    split.
-    split; [constructor |].
-    pred_apply. instantiate (a2:=l); cancel.
-    apply wdiv_lt_upper_bound; [word_neq | rewrite wmult_comm; assumption].
-    apply wmod_upper_bound; word_neq.
-    assumption.
+    intros. eapply pimpl_ok2. eapply RecArray.put_ok; word_neq.
     step.
-    apply pimpl_or_r. right.
-    norm.
-    cancel.
-    split; [constructor |].
-    split; [constructor |].
-    pred_apply. cancel.
-
-    apply upd_divmod.
-    repeat match goal with
-    | [ H: context[rep_pair _ _] |- _ ] =>
-      unfold rep_pair in H; destruct_lift H
-    end.
-    auto.
-
-    admit.
-    admit.
-    admit.
-(*     step. *)
   Qed.
 
   Hint Extern 1 ({{_}} progseq (iget _ _ _) _) => apply iget_ok : prog.
